some hacking with @wildptr

compiler/wasm/stack_to_wasmProofScript.sml
@@ -2,11 +2,51 @@
   Correctness proof for compilation from stackLang to wasmLang
 *)
 Theory stack_to_wasmProof
+Libs
+  preamble helperLib
 Ancestors
   wasmLang words arithmetic list rich_list sptree mlstring
-  wasmSem stackSem stackLang pair
-Libs
-  wordsLib helperLib markerLib BasicProvers
+  wasmSem stackSem stackLang stackProps pair asm
+
+(* TODO: Move to generic automation, perhaps in preamble? *)
+fun component_equality_of ty = let
+  val accfn_terms = map (fn (_, rcd) => #accessor rcd) (TypeBase.fields_of ty)
+  val cases_thm =  TypeBase.nchotomy_of ty
+  val oneone_thm = TypeBase.one_one_of ty
+  val accessor_thms = TypeBase.accessors_of ty
+  val var1 = mk_var("a", ty)
+  val var2 = mk_var("b", ty)
+  val lhs = mk_eq(var1, var2)
+  val rhs_tms =
+    map (fn tm => mk_eq(mk_comb(tm, var1), mk_comb(tm, var2)))
+    accfn_terms
+  val rhs = list_mk_conj rhs_tms
+  val goal = mk_eq(lhs, rhs)
+  val tactic =
+      REPEAT GEN_TAC THEN
+      MAP_EVERY (STRUCT_CASES_TAC o C SPEC cases_thm) [var1, var2] THEN
+      REWRITE_TAC (oneone_thm::accessor_thms)
+  in prove(goal, tactic) end
+
+fun trivial_simps ty = let
+  val t = mk_var ("t", ty)
+  fun f accessor fupd fty =
+    (* fupd (K (accessor t)) *)
+    let val lhs =
+    mk_comb (mk_comb (fupd, mk_comb (mk_const("K",fty-->fty-->fty), mk_comb (accessor, t))), t)
+    in
+    prove (mk_eq (lhs, t), simp[component_equality_of ty])
+    end
+  in
+    map (fn (_, {accessor=accessor, fupd=fupd, ty=ty}) => f accessor fupd ty) (TypeBase.fields_of ty)
+  end
+
+(* BANNED *)
+(*
+val _ = save_thm("state_trivial_simps[simp]", LIST_CONJ (trivial_simps ``:wasmSem$state``));
+*)
+
+Theorem state_trivial_simps[simp] = LIST_CONJ (trivial_simps ``:wasmSem$state``);
 
 (* compiler definition (TODO: move to another file when ready) *)
 
@@ -14,51 +54,67 @@ Libs
 Definition I64_EQ_def:
   I64_EQ = Numeric (N_compare (Eq Int W64))
 End
+
 Definition I64_NE_def:
   I64_NE = Numeric (N_compare (Ne Int W64))
 End
+
 Definition I64_CONST_def:
   I64_CONST w = Numeric (N_const64 Int w)
 End
+
 Definition I32_CONST_def:
   I32_CONST w = Numeric (N_const32 Int w)
 End
+
 Definition I64_ADD_def:
   I64_ADD = Numeric (N_binary (Add Int W64))
 End
+
 Definition I64_SUB_def:
   I64_SUB = Numeric (N_binary (Sub Int W64))
 End
+
 Definition I64_AND_def:
   I64_AND = Numeric (N_binary (And W64))
 End
+
 Definition I64_OR_def:
   I64_OR = Numeric (N_binary (Or W64))
 End
+
 Definition I64_XOR_def:
   I64_XOR = Numeric (N_binary (Xor W64))
 End
+
 Definition I64_SHL_def:
   I64_SHL = Numeric (N_binary (Shl W64))
 End
+
 Definition I64_SHR_S_def:
   I64_SHR_S = Numeric (N_binary (Shr_ Signed W64))
 End
+
 Definition I64_SHR_U_def:
   I64_SHR_U = Numeric (N_binary (Shr_ Unsigned W64))
 End
+
 Definition I64_ROTR_def:
   I64_ROTR = Numeric (N_binary (Rotr W64))
 End
+
 Definition I64_DIV_S_def:
   I64_DIV_S = Numeric (N_binary (Div_ Signed W64))
 End
+
 Definition I64_DIV_U_def:
   I64_DIV_U = Numeric (N_binary (Div_ Unsigned W64))
 End
+
 Definition GLOBAL_GET_def:
   GLOBAL_GET i = Variable (GlobalGet (n2w i))
 End
+
 Definition GLOBAL_SET_def:
   GLOBAL_SET i = Variable (GlobalSet (n2w i))
 End
@@ -125,16 +181,12 @@ Definition compile_arith_def:
 )
 End
 
-
-
 Definition compile_inst_def:
   compile_inst (asm$Skip) = List [] ∧
   compile_inst (asm$Const (r:reg) (v:64 word)) =
     List [I64_CONST v; GLOBAL_SET r] ∧
   compile_inst (asm$Arith a) = compile_arith a
 End
-
-
 
 Definition compile_def:
   compile stackLang$Skip = List ([]:wasmLang$instr list) ∧
@@ -165,22 +217,25 @@ Definition to_value_def:
   to_value (Loc l _) = I64 (n2w l << 1)
 End
 
-Definition regs_rel_def:
-  regs_rel regs globals <=>
-    32 <= LENGTH globals (* no. of avail. regs. of wasm backend *) ∧
-    LENGTH globals < 4294967296 (* 2**32; wasm binary encoding *) ∧
-    ∀n wl. FLOOKUP regs n = SOME wl ==> EL n globals = to_value wl
+Definition conf_ok_def:
+  conf_ok (c: 64 asm_config) ⇔
+  c.reg_count < 4294967296 (* 2**32; wasm binary encoding *)
 End
 
+Definition regs_rel_def:
+  regs_rel c regs globals ⇔
+  LENGTH globals = c.reg_count ∧
+  ∀n wl. FLOOKUP regs n = SOME wl ⇒
+    EL n globals = to_value wl
+End
 
-(* code_rel: we can find long mul at const index i *)
-
+(* TODO: code_rel: we can find long mul at const index i *)
 
 Definition state_rel_def:
-  state_rel ^s ^t ⇔
+  state_rel c ^s ^t ⇔
     ¬ s.use_stack ∧ ¬ s.use_store ∧ ¬ s.use_alloc ∧ ¬ s.be ∧
     empty_buffer s.code_buffer ∧ empty_buffer s.data_buffer ∧
-    regs_rel s.regs t.globals (* ∧ code_rel s.code t.code *)
+    regs_rel c s.regs t.globals (* ∧ code_rel s.code t.code *)
 End
 
 Definition res_rel_def:
@@ -193,12 +248,14 @@ End
 val goal_tm =
   “λ(p,^s). ∀res s1 t.
      evaluate (p,s) = (res,s1) ∧
-     state_rel s t ∧ (* syntax_ok p ∧ *)
+     conf_ok c ∧
+     state_rel c s t ∧
+     stack_asm_ok c p ∧
      res ≠ SOME Error ⇒
      ∃ck t1 res1.
        exec_list (append (compile p)) (t with clock := t.clock + ck) = (res1,t1) ∧
        res_rel res res1 ∧
-       state_rel s1 t1 ∧
+       state_rel c s1 t1 ∧
        (res1 = RNormal ==> t1.stack = t.stack)
   ”
 
@@ -308,6 +365,7 @@ Proof
   Cases_on`e`>>simp[]
 QED
 
+(* wasmProps *)
 Theorem exec_list_add_clock_aux:
 ( ∀c s res s1.
   exec c s = (res,s1) ∧ res ≠ RTimeout ==>
@@ -320,191 +378,191 @@ Theorem exec_list_add_clock_aux:
        (res, s1 with clock := ck + s1.clock)
 )
 Proof
-ho_match_mp_tac exec_ind>>rpt strip_tac
->~[`Unreachable`]
->-fs[exec_def]
->~[`Nop`]
->-fs[exec_def]
->~[`Block`]
->-(
-  qpat_x_assum `exec _ _ = _` mp_tac
-  >>simp[exec_def]
-  >>(pairarg_tac>>fs[])
-  >>(Cases_on`res'=RTimeout`>>gvs[AllCaseEqs()])
-  >>rw[]
-)
->~[‘Loop’]
->-(
-  qpat_x_assum `exec _ _ = _` mp_tac
-  >>once_rewrite_tac[exec_def]
-  >>simp[]
-  >>rpt(pairarg_tac>>fs[])
-  >>(Cases_on`res'=RTimeout`>>gvs[AllCaseEqs()])
-  >>rw[]
-)
->~[‘If’]
->-(
-  qpat_x_assum `exec _ _ = _` mp_tac
-  >>once_rewrite_tac[exec_def]
-  >>simp[CaseEqs["prod","option"]]
-  >>rw[]>-metis_tac[pop_clock]
-  >>fs[]
-  >>metis_tac[pop_clock]
-)
->~[‘Br’]
->-fs[exec_def]
->~[‘BrIf’]
->-(
-  fs[exec_def]
-  >>(Cases_on`s.stack`>>fs[pop_def])
-  >>(PURE_TOP_CASE_TAC>>gvs[state_accfupds])
-  >>(IF_CASES_TAC>>gvs[state_accfupds])
-)
->~[‘BrTable’]
->-(
-  fs[exec_def]
-  >>(Cases_on`s.stack`>>fs[pop_def])
-  >>(PURE_TOP_CASE_TAC>>gvs[state_accfupds])
-)
->~[‘Return’]
->-fs[exec_def]
->~[‘ReturnCall’]
->-(
-  fs[exec_def]
-  >>(PURE_TOP_CASE_TAC>>fs[])
-  >>(PURE_TOP_CASE_TAC>>fs[])
-  >>(PURE_TOP_CASE_TAC>>fs[])
-  >>(Cases_on`pop_n (LENGTH q) s`>>fs[])
-  >>(split_pair_case_tac>>gvs[])
-  >>imp_res_tac pop_n_clock
-  >>(Cases_on`s.clock=0`>>fs[])
-  >>rpt(pairarg_tac>>fs[])
-  >>gvs[AllCaseEqs()]
-)
->~[‘ReturnCallIndirect’]
->-(
-  fs[exec_def]
-  >>(PURE_TOP_CASE_TAC>>gvs[])
-  >>(PURE_TOP_CASE_TAC>>gvs[])
-  >>drule pop_clock
-  >>strip_tac
-  >>rpt(PURE_TOP_CASE_TAC>>gvs[])
-)
->~[‘Call’]
->-(
-  qpat_x_assum`exec _ _ = _`mp_tac
-  >>simp[exec_def]
-  >>(PURE_TOP_CASE_TAC>>fs[])
-  >>(PURE_TOP_CASE_TAC>>fs[])
-  >>(split_pair_case_tac>>gvs[])
-  >>(PURE_TOP_CASE_TAC>>fs[])
-  >>(split_pair_case_tac>>gvs[])
-  >>imp_res_tac pop_n_clock
-  >>gvs[]
-  >>(IF_CASES_TAC>>fs[])
-  >>rpt(pairarg_tac>>fs[])
-  >>(Cases_on`res'=RTimeout`>>fs[])
-  >>first_x_assum $ qspec_then`ck`SUBST_ALL_TAC
-  >>gvs[AllCaseEqs()]
-  >>rw[]
-)
->~[‘CallIndirect’]
->-(
-  qpat_x_assum`exec _ _ = _`mp_tac
-  >>fs[exec_def]
-  >>(PURE_TOP_CASE_TAC>>fs[])
-  >>(split_pair_case_tac>>gvs[])
-  >>imp_res_tac pop_clock
-  >>(PURE_TOP_CASE_TAC>>fs[])>-metis_tac[]
-  >>(PURE_TOP_CASE_TAC>>fs[])
-  >>metis_tac[]
-)
->~[`Numeric`]
->-(
-  fs[exec_def]
-  >>(PURE_TOP_CASE_TAC>>fs[])
-  >>rpt VAR_EQ_TAC
-  >>simp[]
-)
->~[`Parametric Drop`]
->-(
-  fs[exec_def]
-  >>Cases_on`pop s`>>fs[]
-  >>(split_pair_case_tac>>gvs[])
-  >>metis_tac[pop_clock]
-)
->~[`Parametric Select`]
->-(
-  fs[exec_def]
-  >>simp[OPTION_CASE_OPTION_MAP,PAIR_CASE_PAIR_MAP]
-  >>fs[push_def]
-  >>rpt(PURE_TOP_CASE_TAC>>fs[])
-  >>(imp_res_tac pop_clock>>gvs[])
-)
->~[`LocalGet`]
->-(
-  fs[exec_def]
-  >>(PURE_TOP_CASE_TAC>>fs[])
-  >>gvs[push_def]
-)
->~[`LocalSet`]
->-(
-  fs[exec_def]
-  >>simp[OPTION_CASE_OPTION_MAP,PAIR_CASE_PAIR_MAP]
-  >>(PURE_TOP_CASE_TAC>>fs[])
-  >>(split_pair_case_tac>>gvs[])
-  >>imp_res_tac pop_clock
-  >>(PURE_TOP_CASE_TAC>>gvs[])
-  >>metis_tac[set_local_clock]
-)
->~[`LocalTee`]
->-(
-  fs[exec_def]
-  >>simp[OPTION_CASE_OPTION_MAP,PAIR_CASE_PAIR_MAP]
-  >>(PURE_TOP_CASE_TAC>>fs[])
-  >>(split_pair_case_tac>>gvs[])
-  >>imp_res_tac pop_clock
-  >>(PURE_TOP_CASE_TAC>>gvs[])
-  >>metis_tac[set_local_clock]
-)
->~[`GlobalGet`]
->-(
-  fs[exec_def]
-  >>(PURE_TOP_CASE_TAC>>fs[])
-  >>fs[push_def]
-  >>gvs[state_component_equality]
-)
->~[`GlobalSet`]
->-(
-  fs[exec_def]
-  >>simp[OPTION_CASE_OPTION_MAP,PAIR_CASE_PAIR_MAP]
-  >>(PURE_TOP_CASE_TAC>>fs[]>>split_pair_case_tac>>gvs[]>>imp_res_tac pop_clock)
-  >>(PURE_TOP_CASE_TAC>>fs[]>-gvs[state_component_equality])
-  >>metis_tac[set_global_clock]
-)
->~[`MemRead`]
->-(
-  fs[exec_def]
-  >>simp[OPTION_CASE_OPTION_MAP,PAIR_CASE_PAIR_MAP]
-  >>(PURE_TOP_CASE_TAC>>fs[]>>split_pair_case_tac>>gvs[]>>imp_res_tac pop_i32_clock)
-  >>(PURE_TOP_CASE_TAC>>gvs[])
-)
->~[`MemWrite`]
->-(
-  fs[exec_def]
-  >>simp[OPTION_CASE_OPTION_MAP,PAIR_CASE_PAIR_MAP]
-  >>(PURE_TOP_CASE_TAC>>fs[]>>split_pair_case_tac>>gvs[]>>imp_res_tac pop_clock)
-  >>(PURE_TOP_CASE_TAC>>gvs[]>>split_pair_case_tac>>gvs[]>>imp_res_tac pop_i32_clock)
-  >>(PURE_TOP_CASE_TAC>>gvs[])
-)
->-fs[exec_def]
->-(
-  fs[exec_def]
-  >>rpt(pairarg_tac>>fs[])
-  >>(Cases_on`res''=RTimeout`>>fs[])
-  >>first_x_assum $ qspec_then`ck`SUBST_ALL_TAC
-  >>gvs[AllCaseEqs()]
-)
+  ho_match_mp_tac exec_ind>>rpt strip_tac
+  >~[`Unreachable`]
+  >-fs[exec_def]
+  >~[`Nop`]
+  >-fs[exec_def]
+  >~[`Block`]
+  >-(
+    qpat_x_assum `exec _ _ = _` mp_tac
+    >>simp[exec_def]
+    >>(pairarg_tac>>fs[])
+    >>(Cases_on`res'=RTimeout`>>gvs[AllCaseEqs()])
+    >>rw[]
+  )
+  >~[‘Loop’]
+  >-(
+    qpat_x_assum `exec _ _ = _` mp_tac
+    >>once_rewrite_tac[exec_def]
+    >>simp[]
+    >>rpt(pairarg_tac>>fs[])
+    >>(Cases_on`res'=RTimeout`>>gvs[AllCaseEqs()])
+    >>rw[]
+  )
+  >~[‘If’]
+  >-(
+    qpat_x_assum `exec _ _ = _` mp_tac
+    >>once_rewrite_tac[exec_def]
+    >>simp[CaseEqs["prod","option"]]
+    >>rw[]>-metis_tac[pop_clock]
+    >>fs[]
+    >>metis_tac[pop_clock]
+  )
+  >~[‘Br’]
+  >-fs[exec_def]
+  >~[‘BrIf’]
+  >-(
+    fs[exec_def]
+    >>(Cases_on`s.stack`>>fs[pop_def])
+    >>(PURE_TOP_CASE_TAC>>gvs[state_accfupds])
+    >>(IF_CASES_TAC>>gvs[state_accfupds])
+  )
+  >~[‘BrTable’]
+  >-(
+    fs[exec_def]
+    >>(Cases_on`s.stack`>>fs[pop_def])
+    >>(PURE_TOP_CASE_TAC>>gvs[state_accfupds])
+  )
+  >~[‘Return’]
+  >-fs[exec_def]
+  >~[‘ReturnCall’]
+  >-(
+    fs[exec_def]
+    >>(PURE_TOP_CASE_TAC>>fs[])
+    >>(PURE_TOP_CASE_TAC>>fs[])
+    >>(PURE_TOP_CASE_TAC>>fs[])
+    >>(Cases_on`pop_n (LENGTH q) s`>>fs[])
+    >>(split_pair_case_tac>>gvs[])
+    >>imp_res_tac pop_n_clock
+    >>(Cases_on`s.clock=0`>>fs[])
+    >>rpt(pairarg_tac>>fs[])
+    >>gvs[AllCaseEqs()]
+  )
+  >~[‘ReturnCallIndirect’]
+  >-(
+    fs[exec_def]
+    >>(PURE_TOP_CASE_TAC>>gvs[])
+    >>(PURE_TOP_CASE_TAC>>gvs[])
+    >>drule pop_clock
+    >>strip_tac
+    >>rpt(PURE_TOP_CASE_TAC>>gvs[])
+  )
+  >~[‘Call’]
+  >-(
+    qpat_x_assum`exec _ _ = _`mp_tac
+    >>simp[exec_def]
+    >>(PURE_TOP_CASE_TAC>>fs[])
+    >>(PURE_TOP_CASE_TAC>>fs[])
+    >>(split_pair_case_tac>>gvs[])
+    >>(PURE_TOP_CASE_TAC>>fs[])
+    >>(split_pair_case_tac>>gvs[])
+    >>imp_res_tac pop_n_clock
+    >>gvs[]
+    >>(IF_CASES_TAC>>fs[])
+    >>rpt(pairarg_tac>>fs[])
+    >>(Cases_on`res'=RTimeout`>>fs[])
+    >>first_x_assum $ qspec_then`ck`SUBST_ALL_TAC
+    >>gvs[AllCaseEqs()]
+    >>rw[]
+  )
+  >~[‘CallIndirect’]
+  >-(
+    qpat_x_assum`exec _ _ = _`mp_tac
+    >>fs[exec_def]
+    >>(PURE_TOP_CASE_TAC>>fs[])
+    >>(split_pair_case_tac>>gvs[])
+    >>imp_res_tac pop_clock
+    >>(PURE_TOP_CASE_TAC>>fs[])>-metis_tac[]
+    >>(PURE_TOP_CASE_TAC>>fs[])
+    >>metis_tac[]
+  )
+  >~[`Numeric`]
+  >-(
+    fs[exec_def]
+    >>(PURE_TOP_CASE_TAC>>fs[])
+    >>rpt VAR_EQ_TAC
+    >>simp[]
+  )
+  >~[`Parametric Drop`]
+  >-(
+    fs[exec_def]
+    >>Cases_on`pop s`>>fs[]
+    >>(split_pair_case_tac>>gvs[])
+    >>metis_tac[pop_clock]
+  )
+  >~[`Parametric Select`]
+  >-(
+    fs[exec_def]
+    >>simp[OPTION_CASE_OPTION_MAP,PAIR_CASE_PAIR_MAP]
+    >>fs[push_def]
+    >>rpt(PURE_TOP_CASE_TAC>>fs[])
+    >>(imp_res_tac pop_clock>>gvs[])
+  )
+  >~[`LocalGet`]
+  >-(
+    fs[exec_def]
+    >>(PURE_TOP_CASE_TAC>>fs[])
+    >>gvs[push_def]
+  )
+  >~[`LocalSet`]
+  >-(
+    fs[exec_def]
+    >>simp[OPTION_CASE_OPTION_MAP,PAIR_CASE_PAIR_MAP]
+    >>(PURE_TOP_CASE_TAC>>fs[])
+    >>(split_pair_case_tac>>gvs[])
+    >>imp_res_tac pop_clock
+    >>(PURE_TOP_CASE_TAC>>gvs[])
+    >>metis_tac[set_local_clock]
+  )
+  >~[`LocalTee`]
+  >-(
+    fs[exec_def]
+    >>simp[OPTION_CASE_OPTION_MAP,PAIR_CASE_PAIR_MAP]
+    >>(PURE_TOP_CASE_TAC>>fs[])
+    >>(split_pair_case_tac>>gvs[])
+    >>imp_res_tac pop_clock
+    >>(PURE_TOP_CASE_TAC>>gvs[])
+    >>metis_tac[set_local_clock]
+  )
+  >~[`GlobalGet`]
+  >-(
+    fs[exec_def]
+    >>(PURE_TOP_CASE_TAC>>fs[])
+    >>fs[push_def]
+    >>gvs[state_component_equality]
+  )
+  >~[`GlobalSet`]
+  >-(
+    fs[exec_def]
+    >>simp[OPTION_CASE_OPTION_MAP,PAIR_CASE_PAIR_MAP]
+    >>(PURE_TOP_CASE_TAC>>fs[]>>split_pair_case_tac>>gvs[]>>imp_res_tac pop_clock)
+    >>(PURE_TOP_CASE_TAC>>fs[]>-gvs[state_component_equality])
+    >>metis_tac[set_global_clock]
+  )
+  >~[`MemRead`]
+  >-(
+    fs[exec_def]
+    >>simp[OPTION_CASE_OPTION_MAP,PAIR_CASE_PAIR_MAP]
+    >>(PURE_TOP_CASE_TAC>>fs[]>>split_pair_case_tac>>gvs[]>>imp_res_tac pop_i32_clock)
+    >>(PURE_TOP_CASE_TAC>>gvs[])
+  )
+  >~[`MemWrite`]
+  >-(
+    fs[exec_def]
+    >>simp[OPTION_CASE_OPTION_MAP,PAIR_CASE_PAIR_MAP]
+    >>(PURE_TOP_CASE_TAC>>fs[]>>split_pair_case_tac>>gvs[]>>imp_res_tac pop_clock)
+    >>(PURE_TOP_CASE_TAC>>gvs[]>>split_pair_case_tac>>gvs[]>>imp_res_tac pop_i32_clock)
+    >>(PURE_TOP_CASE_TAC>>gvs[])
+  )
+  >-fs[exec_def]
+  >-(
+    fs[exec_def]
+    >>rpt(pairarg_tac>>fs[])
+    >>(Cases_on`res''=RTimeout`>>fs[])
+    >>first_x_assum $ qspec_then`ck`SUBST_ALL_TAC
+    >>gvs[AllCaseEqs()]
+  )
 QED
 
 Theorem exec_list_add_clock:
@@ -519,7 +577,7 @@ Theorem comp_cmp_thm:
   get_var a s = SOME va ∧
   get_var_imm b s = SOME vb ∧
   labSem$word_cmp cmp va vb = SOME v ∧
-  state_rel ^s ^t ==>
+  state_rel c ^s ^t ==>
   exec_list (append (comp_cmp cmp a b)) (t with clock := ck) =
     (RNormal, push (I32 (b2w v)) (t with clock := ck))
 Proof
@@ -549,98 +607,93 @@ Proof
   \\ qexists_tac ‘0’ \\ fs [state_rel_def]
 QED
 
-fun component_equality_of ty = let
-val accfn_terms = map (fn (_, rcd) => #accessor rcd) (TypeBase.fields_of ty)
-val cases_thm =  TypeBase.nchotomy_of ty
-val oneone_thm = TypeBase.one_one_of ty
-val accessor_thms = TypeBase.accessors_of ty
-    val var1 = mk_var("a", ty)
-    val var2 = mk_var("b", ty)
-    val lhs = mk_eq(var1, var2)
-    val rhs_tms =
-      map (fn tm => mk_eq(mk_comb(tm, var1), mk_comb(tm, var2)))
-      accfn_terms
-    val rhs = list_mk_conj rhs_tms
-    val goal = mk_eq(lhs, rhs)
-    val tactic =
-      REPEAT GEN_TAC THEN
-      MAP_EVERY (STRUCT_CASES_TAC o C SPEC cases_thm) [var1, var2] THEN
-      REWRITE_TAC (oneone_thm::accessor_thms)
-    in prove(goal, tactic) end
+Theorem exec_I64_CONST:
+  exec (I64_CONST c) s =
+    (RNormal,s with stack := I64 c::s.stack)
+Proof
+  rw[exec_def,I64_CONST_def,num_stk_op_def]
+QED
 
-fun trivial_simps ty =
-let
-val t = mk_var ("t", ty)
-fun f accessor fupd fty =
-(* fupd (K (accessor t)) *)
-let val lhs =
-mk_comb (mk_comb (fupd, mk_comb (mk_const("K",fty-->fty-->fty), mk_comb (accessor, t))), t)
-in
-prove (mk_eq (lhs, t), simp[component_equality_of ty])
-end
-in
-map (fn (_, {accessor=accessor, fupd=fupd, ty=ty}) => f accessor fupd ty) (TypeBase.fields_of ty)
-end
+Theorem exec_GLOBAL_SET:
+  exec (GLOBAL_SET n) s = (res,s') ∧
+  n < LENGTH s.globals ∧
+  LENGTH s.globals < 4294967296 ∧
+  s.stack = v :: t ⇒
+  res = RNormal ∧
+  s' = s with
+     <|stack := t;
+       globals := LUPDATE v n s.globals|>
+Proof
+  rw[exec_def,GLOBAL_SET_def,pop_def,set_global_def]>>
+  gvs[AllCaseEqs()]
+QED
 
-(* BANNED *)
-(*
-val _ = save_thm("state_trivial_simps[simp]", LIST_CONJ (trivial_simps ``:wasmSem$state``));
-*)
+Theorem exec_list_Nil[simp]:
+  exec_list [] s = (RNormal,s)
+Proof
+  rw[exec_def]
+QED
 
-Theorem state_trivial_simps[simp] = LIST_CONJ (trivial_simps ``:wasmSem$state``);
+Theorem state_rel_set_var:
+  to_value v = w ∧
+  n < LENGTH t.globals ∧
+  state_rel c s t ⇒
+  state_rel c (set_var n v s)
+    (t with globals := LUPDATE w n t.globals)
+Proof
+  rw[state_rel_def,regs_rel_def,EL_LUPDATE,set_var_def]>>
+  fs[FLOOKUP_UPDATE]>>
+  rw[]>>
+  gvs[AllCaseEqs()]
+QED
+
+Theorem state_trivial_2_simps[simp]:
+  s with <| stack := s.stack ; globals := g |> =
+  s with <| globals := g |>
+Proof
+  rw[wasmSemTheory.state_component_equality]
+QED
 
 Theorem compile_Inst:
   ^(get_goal "Inst")
 Proof
-rw[compile_def]
->>qexists_tac`0`
->>(Cases_on`i`>>fs[compile_inst_def])
->-(
-  fs[evaluate_def,inst_def]
-  >>fs[exec_def,res_rel_def]
-  >>gvs[]
-)
-(* Const *)
->-(
-  fs[evaluate_def,inst_def]
-  >>fs[assign_def]
-  >>gvs[CaseEq"option"]
-  >>fs[exec_list_cons]
-  >>rpt(pairarg_tac>>fs[])
-  >>rename1`exec (I64_CONST c) t = (res1,t1)`
-  >>rename1`exec (GLOBAL_SET n) t1 = (res2,t2)`
-  >>subgoal`res1=RNormal∧res2=RNormal`
-  >-(
-    fs[I64_CONST_def,GLOBAL_SET_def,exec_def]
-    >>gvs[num_stk_op_def]
-    >>fs[pop_def]
-    >>fs[set_global_def]
-    >>`n MOD 4294967296 < LENGTH t.globals` by cheat (* use names_ok? stack_asm_name? *)
-    >>fs[]
-  )
-  >>fs[exec_def,res_rel_def]
-  (*
-      0.  word_exp s (Const c) = SOME w
-      1.  state_rel s t
-      2.  exec (I64_CONST c) t = (RNormal,t1)
-      3.  exec (GLOBAL_SET n) t1 = (RNormal,t2)
-      4.  res1 = RNormal
-      5.  res2 = RNormal
-     ------------------------------------
-          state_rel (set_var n (Word w) s) t2 ∧ t2.stack = t.stack
-  *)
-  >>fs[I64_CONST_def,GLOBAL_SET_def,exec_def]
-  >>gvs[AllCaseEqs()]
-  >>gvs[num_stk_op_def]
-  >>gvs[pop_def]
-  >>gvs[set_global_def]
-  `n < LENGTH t.globals` by cheat(*syntactic*)
-`LENGTH t.globals < 4294967296` by cheat(*global*)
-
-
-  >>cheat
-)
-
+  rw[compile_def]
+  >>qexists_tac`0`
+  >>(Cases_on`i`>>fs[compile_inst_def])
+  >~[`Skip`]>-
+    gvs[evaluate_def,exec_def,res_rel_def,inst_def]
+  >~[`Const`]>- (
+    fs[evaluate_def,inst_def,assign_def,CaseEq"option"]
+    >>fs[exec_list_cons,exec_I64_CONST]
+    >>rpt(pairarg_tac>>fs[])
+    >> drule exec_GLOBAL_SET
+    >> simp[]
+    >> impl_keep_tac >-
+      fs[stack_asm_ok_def,inst_ok_def,reg_ok_def,conf_ok_def,state_rel_def,regs_rel_def]>>
+    rw[]
+    >-
+      simp[res_rel_def]>>
+    irule state_rel_set_var>>
+    fs[word_exp_def,to_value_def])
+  >~[`Arith`] >- (
+    rename1`Arith a`>>Cases_on`a`
+    >~[`Binop`] >- cheat
+    >~[`Shift`] >- cheat
+    >~[`Div`] >- cheat
+    >~[`LongMul`] >- cheat
+    >~[`LongDiv`] >-
+      (* TODO: is there an explicit invariant that
+        bans this? *)
+      cheat
+    >~[`AddCarry`] >- cheat
+    >~[`AddOverflow`] >- cheat
+    >~[`SubOverflow`] >- cheat
+    )
+  >~[`Mem`] >-
+    cheat
+  >~[`FP`] >- (
+    fs[stack_asm_ok_def,inst_ok_def,fp_ok_def]>>
+    cheat)
 QED
 
 Theorem compile_Seq:
@@ -655,14 +708,14 @@ Proof
   >>rename[‘_ = (res_mid, s_mid)’]
   >>reverse $ Cases_on‘res_mid’
   >-(
-    gvs[]
+    gvs[stack_asm_ok_def]
     >>last_x_assum drule
     >>strip_tac
     >>qexists_tac‘ck’
     >>simp[]
     >>fs[res_rel_def]
   )
-  >>gvs[]
+  >>gvs[stack_asm_ok_def]
   >>last_x_assum $ ASSUME_NAMED_TAC "H1"
   >>qpat_x_assum ‘∀t'. _’ $ ASSUME_NAMED_TAC "H2"
   >>LABEL_X_ASSUM "H2" drule
@@ -677,18 +730,17 @@ Proof
 QED
 
 Theorem state_rel_with_stack:
-  state_rel s (t with stack := st) = state_rel s t
+  state_rel c s (t with stack := st) = state_rel c s t
 Proof
   fs[state_rel_def]
 QED
-(* delsimps["state_rel_with_stack"] *)
 
 Theorem compile_If:
   ^(get_goal "If")
 Proof
   rpt strip_tac
   >> fs[evaluate_def]
-  >> gvs[CaseEq"option"]
+  >> gvs[CaseEq"option",stack_asm_ok_def]
   >> simp[compile_def]
   >> simp[exec_list_append]
   >> drule_all comp_cmp_thm
@@ -697,7 +749,7 @@ Proof
   >> pop_assum kall_tac
   >> simp[exec_def,pop_push]
   >> simp[nonzero_b2w]
-  >> ‘state_rel s (t with stack:=[])’ by simp[state_rel_with_stack]
+  >> ‘state_rel c s (t with stack:=[])’ by simp[state_rel_with_stack]
   >> IF_CASES_TAC>>gvs[]>>first_x_assum drule>>strip_tac
   >> (
     qexists_tac‘ck’
